theories/Core/Semantic/NbE.v
@@ -6,20 +6,20 @@ Import Domain_Notations.
 
 Generalizable All Variables.
 
-Inductive initial_env {P : PtsSig} : ctx P -> env P -> Prop :=
-| initial_env_nil : initial_env nil empty_env
+Inductive initial_env {P : PtsSig} : gctx P -> ctx P -> env P -> Prop :=
+| initial_env_nil : initial_env nil nil empty_env
 | initial_env_cons :
-  `( initial_env Γ ρ ->
-     {{ ⟦ A ⟧ ρ ↘ a }} ->
-     initial_env ({{{ Γ, A }}}) d{{{ ρ ↦ ⇑! a (length Γ) }}}).
+  `( initial_env Δ Γ ρ ->
+     {{ ⟦ A ⟧ (Δ ; ρ) ↘ a }} ->
+     initial_env Δ ({{{ Γ, A }}}) d{{{ ρ ↦ ⇑! a (length Γ) }}}).
 
 #[export]
 Hint Constructors initial_env : mcpts.
 
-Lemma functional_initial_env {P : PtsSig} : forall (Γ : ctx P) ρ,
-    initial_env Γ ρ ->
+Lemma functional_initial_env {P : PtsSig} : forall (Δ : gctx P) Γ ρ,
+    initial_env Δ Γ ρ ->
     forall ρ',
-      initial_env Γ ρ' ->
+      initial_env Δ Γ ρ' ->
       ρ = ρ'.
 Proof.
   induction 1; intros ? Hother; inversion_clear Hother; eauto.
@@ -35,8 +35,8 @@ Hint Resolve functional_initial_env : mcpts.
     whether [a] is the evaluation result of A or not.
     If we want to specify that as well, we need a generalized
     version of [drop_env] that can drop [x] elements. *)
-Lemma initial_env_spec {P : PtsSig} : forall x (Γ : ctx P) ρ A,
-    initial_env Γ ρ ->
+Lemma initial_env_spec {P : PtsSig} : forall x (Δ : gctx P) Γ ρ A,
+    initial_env Δ Γ ρ ->
     {{ #x : A ∈ Γ }} ->
     exists m a, {{ #| ρ[x] |↘ m }} /\ m = d{{{ ⇑! a (length Γ - x - 1) }}}.
 Proof.
@@ -58,8 +58,8 @@ Qed.
 #[export]
 Hint Resolve initial_env_spec : mcpts.
 
-Lemma initial_env_spec_subst {P} : forall x (Γ : ctx P) ρ A,
-    initial_env Γ ρ ->
+Lemma initial_env_spec_subst {P} : forall x (Δ : gctx P) Γ ρ A,
+    initial_env Δ Γ ρ ->
     {{ #x : A ∈ Γ }} ->
     exists a, {{ #| ρ[x] |↘ ⇑! a (length Γ - x - 1) }}.
 Proof.
@@ -76,26 +76,26 @@ Hint Resolve initial_env_spec_subst : mcpts.
 Ltac functional_initial_env_rewrite_clear1 :=
   let tactic_error o1 o2 := fail 3 "functional_initial_env equality between" o1 "and" o2 "cannot be solved by mauto" in
   match goal with
-  | H1 : initial_env ?G ?ρ, H2 : initial_env ?G ?ρ' |- _ =>
+  | H1 : initial_env ?Δ ?Γ ?ρ, H2 : initial_env ?Δ ?Γ ?ρ' |- _ =>
       clean replace ρ' with ρ by first [solve [mauto 2] | tactic_error ρ' ρ]; clear H2
   end.
 Ltac functional_initial_env_rewrite_clear := repeat functional_initial_env_rewrite_clear1.
 
-Inductive nbe {P : PtsSig} : ctx P -> exp P -> typ P -> nf P -> Prop :=
+Inductive nbe {P : PtsSig} : gctx P -> ctx P -> exp P -> typ P -> nf P -> Prop :=
 | nbe_run :
-  `( initial_env Γ ρ ->
-     {{ ⟦ A ⟧ ρ ↘ a }} ->
-     {{ ⟦ M ⟧ ρ ↘ m }} ->
-     {{ Rnf ⇓ a m in (length Γ) ↘ w }} ->
-     nbe Γ M A w ).
+  `( initial_env Δ Γ ρ ->
+     {{ ⟦ A ⟧ (Δ ; ρ) ↘ a }} ->
+     {{ ⟦ M ⟧ (Δ ; ρ) ↘ m }} ->
+     {{ Rnf ⇓ a m in (length Γ) ↘ W }} ->
+     nbe Δ Γ M A W ).
 
 #[export]
 Hint Constructors nbe : mcpts.
 
-Lemma functional_nbe {P : PtsSig} : forall (Γ : ctx P) M A w w',
-    nbe Γ M A w ->
-    nbe Γ M A w' ->
-    w = w'.
+Lemma functional_nbe {P : PtsSig} : forall (Δ : gctx P) Γ M A W W',
+    nbe Δ Γ M A W ->
+    nbe Δ Γ M A W' ->
+    W = W'.
 Proof.
   intros.
   inversion_clear H; inversion_clear H0;
@@ -108,20 +108,20 @@ Qed.
 #[export]
 Hint Resolve functional_nbe : mcpts.
 
-Inductive nbe_ty {P : PtsSig} : ctx P -> typ P -> nf P -> Prop :=
+Inductive nbe_ty {P : PtsSig} : gctx P -> ctx P -> typ P -> nf P -> Prop :=
 | nbe_ty_run :
-  `( initial_env Γ ρ ->
-     {{ ⟦ M ⟧ ρ ↘ m }} ->
+  `( initial_env Δ Γ ρ ->
+     {{ ⟦ M ⟧ (Δ ; ρ) ↘ m }} ->
      {{ Rtyp m in (length Γ) ↘ W }} ->
-     nbe_ty Γ M W ).
+     nbe_ty Δ Γ M W ).
 
 #[export]
 Hint Constructors nbe_ty : mcpts.
 
-Lemma functional_nbe_ty {P : PtsSig} : forall (Γ : ctx P) M w w',
-    nbe_ty Γ M w ->
-    nbe_ty Γ M w' ->
-    w = w'.
+Lemma functional_nbe_ty {P : PtsSig} : forall (Δ : gctx P) Γ M W W',
+    nbe_ty Δ Γ M W ->
+    nbe_ty Δ Γ M W' ->
+    W = W'.
 Proof.
   intros.
   inversion_clear H; inversion_clear H0;
@@ -131,25 +131,39 @@ Proof.
   reflexivity.
 Qed.
 
-Lemma nbe_type_to_nbe_ty {P : PtsSig} : forall (Γ : ctx P) M s w,
-    nbe Γ M {{{ Sort@s }}} w ->
-    nbe_ty Γ M w.
+#[export]
+Hint Resolve functional_nbe_ty : mcpts.
+  
+Lemma nbe_type_to_nbe_ty {P : PtsSig} : forall (Δ : gctx P) Γ M s W,
+    nbe Δ Γ M {{{ Sort@s }}} W ->
+    nbe_ty Δ Γ M W.
 Proof.
   intros. progressive_inversion.
   mauto.
 Qed.
 
 #[export]
-Hint Resolve functional_nbe_ty nbe_type_to_nbe_ty : mcpts.
+Hint Resolve nbe_type_to_nbe_ty : mcpts.
+
+Lemma function_nbe_nbe_ty {P : PtsSig} : forall (Δ : gctx P) Γ A s W W',
+    nbe Δ Γ A {{{ Sort@s }}} W ->
+    nbe_ty Δ Γ A W' ->
+    W = W'.
+Proof.
+  intros * ?%nbe_type_to_nbe_ty ?.
+  mauto 2.
+Qed.
 
 Ltac functional_nbe_rewrite_clear1 :=
   let tactic_error o1 o2 := fail 3 "functional_nbe equality between" o1 "and" o2 "cannot be solved by mauto" in
   match goal with
-  | H1 : nbe ?G ?M ?A ?W, H2 : nbe ?G ?M ?A ?W' |- _ =>
+  | H1 : nbe ?Δ ?Γ ?M ?A ?W, H2 : nbe ?Δ ?Γ ?M ?A ?W' |- _ =>
       clean replace W' with W by first [solve [mauto 2] | tactic_error W' W]; clear H2
-  | H1 : nbe ?G ?A {{{ Sort@?s }}} ?W, H2 : nbe ?G ?A {{{ Sort@?s }}} ?W' |- _ =>
+  | H1 : nbe ?Δ ?Γ ?A {{{ Sort@?s }}} ?W, H2 : nbe ?Δ ?Γ ?A {{{ Sort@?s }}} ?W' |- _ =>
+      clean replace W' with W by first [solve [mauto 2] | tactic_error W' W]; clear H2
+  | H1 : nbe_ty ?Δ ?Γ ?M ?W, H2 : nbe_ty ?Δ ?Γ ?M ?W' |- _ =>
+      clean replace W' with W by first [solve [mauto 2] | tactic_error W' W]; clear H2
+  | H1 : nbe ?Δ ?Γ ?A {{{ Sort@?s }}} ?W, H2 : nbe_ty ?Δ ?Γ ?A ?W' |- _ =>
       clean replace W' with W by first [solve [mauto 2] | tactic_error W' W]
-  | H1 : nbe_ty ?G ?M ?W, H2 : nbe_ty ?G ?M ?W' |- _ =>
-      clean replace W' with W by first [solve [mauto 2] | tactic_error W' W]; clear H2
   end.
 Ltac functional_nbe_rewrite_clear := repeat functional_nbe_rewrite_clear1.
